Finish refactoring icompile

compiler/backend/icompile/ibackendScript.sml
@@ -1856,6 +1856,17 @@ Proof
   rw[config_prog_rel_b2b_def]
 QED
 
+Theorem bvi_to_data_prog_compile_append_all:
+  bvi_to_data$compile_prog (bvi_init ++ icompiled_p_bvi ++ bvi_end) =
+  bvi_to_data$compile_prog bvi_init ++
+  bvi_to_data$compile_prog icompiled_p_bvi ++
+  bvi_to_data$compile_prog bvi_end
+Proof
+  rw[bvi_to_dataTheory.compile_prog_def] >> gvs[]
+QED
+
+
+
 Theorem init_icompile_icompile_end_icompile_f2c_alt:
   init_icompile_source_to_flat source_conf = (source_iconf, flat_stub) ⇒
   flat_to_clos$compile_prog (flat_stub ++ icompiled_p_flat) =
@@ -1865,10 +1876,29 @@ Proof
 QED
 
 
+
+
+Theorem init_icompile_icompile_end_icompile_d2w0:
+  init_icompile_data_to_word data_conf asm_conf data_init = (data_conf', word0_stub)
+  ⇒
+  (let icompiled_p_word0 = icompile_data_to_word data_conf' icompiled_p_data in
+   let word0_end = icompile_data_to_word data_conf' data_end in
+   data_to_word$compile_0 data_conf asm_conf (data_init ++ icompiled_p_data ++ data_end)
+   =
+   word0_stub ++ icompiled_p_word0 ++ word0_end)
+Proof
+  rw[init_icompile_data_to_word_def,
+     data_to_wordTheory.compile_0_def,
+     icompile_data_to_word_def]
+QED
+
+
 Definition word_conf_ok_def:
   word_conf_ok word_conf =
   (word_conf.col_oracle = [])
 End
+
+
 
 (* for some reason if i dont use a, b, c , i cannot qpat *)
 Theorem init_icompile_icompile_end_icompile_d2w1:
@@ -2108,25 +2138,85 @@ Proof
 QED
 
 
-Definition config_prog_rel_livesets:
-  config_prog_rel_livesets a a'
-                           b b'
-                           c c'
-                           d d'
-                           e e'
-                           f f'=
-  (a = a' ∧
-  b = b' ∧
-  c = c' ∧
-  d = d' ∧
-  e = e' ∧ f = f')
-
-End
-
 (* livesets *)
 
-Definition icompile_to_livesets_def:
-  icompile_to_livesets source_iconf clos_iconf bvl_iconf data_conf word_conf asm_conf p =
+
+Definition source_to_word0_def:
+  source_to_word0 asm_conf (c : mconfig) p =
+  let source_conf = c.source_conf in
+  let clos_conf = c.clos_conf in
+  let bvl_conf = c.bvl_conf in
+  let data_conf = c.data_conf in
+  let p = source_to_source$compile p in
+  let (source_conf', compiled_p_flat) =
+    source_to_flat$compile source_conf p in
+  let compiled_p_clos =
+    flat_to_clos$compile_prog compiled_p_flat in
+  let (clos_conf', compiled_p_bvl) =
+    clos_to_bvl_compile_alt clos_conf compiled_p_clos in
+  let (clos_conf', bvl_conf', compiled_p_bvi) =
+    bvl_to_bvi_compile_update_config clos_conf' bvl_conf compiled_p_bvl in
+  let compiled_p_data =
+    bvi_to_data$compile_prog compiled_p_bvi in
+  let p_word0 = data_to_word$compile_0 data_conf asm_conf compiled_p_data in
+  let c' = c with <| source_conf := source_conf';
+                     clos_conf := clos_conf';
+                     bvl_conf := bvl_conf' |> in
+    (c', p_word0)
+End
+
+
+Definition word0_to_livesets_def:
+  word0_to_livesets asm_conf (word_to_word_conf, p) =
+  let alg = word_to_word_conf.reg_alg in
+  let p =
+    MAP (λ(name_num,arg_count,prog).
+    let prog = word_simp$compile_exp prog in
+    let maxv = max_var prog + 1 in
+    let inst_prog = inst_select asm_conf maxv prog in
+    let ssa_prog = full_ssa_cc_trans arg_count inst_prog in
+    let rm_ssa_prog = remove_dead_prog ssa_prog in
+    let cse_prog = word_common_subexp_elim rm_ssa_prog in
+    let cp_prog = copy_prop cse_prog in
+    let two_prog = three_to_two_reg_prog asm_conf.two_reg_arith cp_prog in
+    let unreach_prog = remove_unreach two_prog in
+    let rm_prog = remove_dead_prog unreach_prog in
+        (name_num,arg_count,rm_prog))
+      p in
+    let data = MAP (\(name_num,arg_count,prog).
+    let (heu_moves,spillcosts) = get_heuristics alg name_num prog in
+    (get_clash_tree prog,heu_moves,spillcosts,
+      get_forced asm_conf prog [],get_stack_only prog)) p
+  in
+    ((asm_conf.reg_count - (5+LENGTH asm_conf.avoid_regs),data), p)
+End
+
+Definition source_to_livesets_def:
+  source_to_livesets asm_conf c p =
+  let (c', pword0) = source_to_word0 asm_conf c p in
+  let ((reg_count, data), pword) = word0_to_livesets asm_conf (c.word_to_word_conf, pword0) in
+    (c', (reg_count, data), pword)
+End
+
+
+
+
+Theorem word0_to_livesets_append:
+  word0_to_livesets asm_conf (word_conf, p1) = ((a, data1), p1') ∧
+  word0_to_livesets asm_conf (word_conf, p2) = ((_, data2), p2') ⇒
+  word0_to_livesets asm_conf (word_conf, (p1 ++ p2)) = ((a, data1 ++ data2), p1' ++ p2')
+Proof
+  rw[word0_to_livesets_def]
+QED
+
+
+Definition icompile_source_to_livesets_def:
+  icompile_source_to_livesets asm_conf (ic: 'a iconfig) p =
+  let source_iconf = ic.source_iconf in
+  let clos_iconf = ic.clos_iconf in
+  let bvl_iconf = ic.bvl_iconf in
+  let data_conf = ic.data_conf in
+  let word_to_word_conf = ic.word_to_word_conf in
   let p = source_to_source$compile p in
   case icompile_source_to_flat source_iconf p of NONE => NONE
   | SOME (source_iconf', icompiled_p_flat) =>
@@ -2134,252 +2224,208 @@ Definition icompile_to_livesets_def:
   let (clos_iconf', icompiled_p_bvl) = icompile_clos_to_bvl_alt clos_iconf icompiled_p_clos in
   let (bvl_iconf', icompiled_p_bvi) = icompile_bvl_to_bvi bvl_iconf icompiled_p_bvl in
   let icompiled_p_data = bvi_to_data$compile_prog icompiled_p_bvi in
-  let icompiled_p_word = icompile_data_to_word data_conf icompiled_p_data in
-  let ((reg_count , data), icompiled_p_livesets) = to_livesets_0_alt asm_conf (word_conf, icompiled_p_word) in
-    SOME (source_iconf', clos_iconf', bvl_iconf', data, icompiled_p_livesets)
+  let icompiled_p_word0 = icompile_data_to_word data_conf icompiled_p_data in
+  let ((reg_count, data), pword0) = word0_to_livesets asm_conf (word_to_word_conf, icompiled_p_word0) in
+  let ic' = ic with <| source_iconf := source_iconf';
+                      clos_iconf := clos_iconf';
+                      bvl_iconf := bvl_iconf'; |> in
+    SOME (ic', data, pword0: (num # num # 'a prog) list)
 End
 
-Definition fold_icompile_to_livesets_def:
-  fold_icompile_to_livesets source_iconf clos_iconf bvl_iconf data_conf word_conf asm_conf []  =
-  icompile_to_livesets source_iconf clos_iconf bvl_iconf data_conf word_conf asm_conf []
-  ∧
-  fold_icompile_to_livesets source_iconf clos_iconf bvl_iconf data_conf word_conf asm_conf (p :: ps)  =
-  case icompile_to_livesets source_iconf clos_iconf bvl_iconf data_conf word_conf asm_conf p  of NONE => NONE
-  | SOME (source_iconf', clos_iconf', bvl_iconf', livesets_data', p') =>
-    (case fold_icompile_to_livesets source_iconf' clos_iconf' bvl_iconf' data_conf word_conf asm_conf ps of NONE => NONE
-    | SOME (source_iconf'', clos_iconf'', bvl_iconf'', livesets_data'', ps') =>
-      SOME (source_iconf'', clos_iconf'', bvl_iconf'', livesets_data' ++ livesets_data'', p' ++ ps'))
-End
-
-Definition init_icompile_to_livesets_def:
-  init_icompile_to_livesets source_conf clos_conf bvl_conf data_conf word_conf asm_conf =
+Definition init_icompile_source_to_livesets_def:
+  init_icompile_source_to_livesets (asm_conf: 'a asm_config) (c: mconfig) =
+  let source_conf = c.source_conf in
+  let clos_conf = c.clos_conf in
+  let bvl_conf = c.bvl_conf in
+  let data_conf = c.data_conf in
+  let word_to_word_conf = c.word_to_word_conf in
   let (source_iconf, flat_stub) = init_icompile_source_to_flat source_conf in
   let clos_stub = init_icompile_flat_to_clos flat_stub in
   let (clos_iconf, bvl_init) = init_icompile_clos_to_bvl clos_conf clos_stub in
   let (bvl_iconf, bvi_init) = init_icompile_bvl_to_bvi bvl_conf bvl_init in
   let data_init = bvi_to_data$compile_prog bvi_init in
-  let (data_conf, word_init) = init_icompile_data_to_word data_conf asm_conf data_init in
-  let ((reg_count, data), livesets_init) = to_livesets_0_alt asm_conf (word_conf, word_init) in
-    (source_iconf, clos_iconf, bvl_iconf, data_conf, (reg_count, data), livesets_init)
+  let (data_conf', word0_init) = init_icompile_data_to_word data_conf asm_conf data_init in
+  let ((reg_count, data), word0_init_lvs) = word0_to_livesets asm_conf (word_to_word_conf, word0_init) in
+  let ic = <| source_iconf := source_iconf;
+              clos_iconf := clos_iconf;
+              bvl_iconf := bvl_iconf;
+              data_conf := data_conf';
+              word_to_word_conf := word_to_word_conf;
+           |>
+  in
+    (ic, (reg_count, data), word0_init_lvs)
 End
 
-Definition end_icompile_to_livesets_def:
-  end_icompile_to_livesets source_iconf source_conf
-                           clos_iconf clos_conf
-                           bvl_iconf bvl_conf
-                           data_conf word_conf asm_conf
+
+Definition end_icompile_source_to_livesets_def:
+  end_icompile_source_to_livesets asm_conf ic (c : mconfig)
   =
+  let source_iconf = ic.source_iconf in
+  let clos_iconf = ic.clos_iconf in
+  let bvl_iconf = ic.bvl_iconf in
+  let data_conf = ic.data_conf in
+  let word_to_word_conf = ic.word_to_word_conf in
+  let source_conf = c.source_conf in
+  let clos_conf = c.clos_conf in
+  let bvl_conf = c.bvl_conf in
   let source_conf_after_ic = end_icompile_source_to_flat source_iconf source_conf in
   let (clos_conf_after_ic, bvl_end) = end_icompile_clos_to_bvl clos_iconf clos_conf in
   let (clos_conf_after_ic_bvi, bvl_conf_after_ic, bvi_end) =
       end_icompile_bvl_to_bvi bvl_end bvl_iconf clos_conf_after_ic bvl_conf in
   let data_end = bvi_to_data$compile_prog bvi_end in
-  let word_end = icompile_data_to_word data_conf data_end in
-  let ((reg_count, data), livesets_end) = to_livesets_0_alt asm_conf (word_conf, word_end) in
-    (source_conf_after_ic, clos_conf_after_ic_bvi, bvl_conf_after_ic, data, livesets_end)
+  let word0_end = icompile_data_to_word data_conf data_end in
+  let ((reg_count, data), word0_end_lvs) = word0_to_livesets asm_conf (word_to_word_conf, word0_end) in
+  let c' = c with
+             <| source_conf := source_conf_after_ic;
+                clos_conf := clos_conf_after_ic_bvi;
+                bvl_conf := bvl_conf_after_ic |> in
+    (c', data, word0_end_lvs)
 End
 
 
-
-Theorem init_icompile_icompile_end_icompile_to_livesets:
-  init_icompile_to_livesets source_conf clos_conf bvl_conf data_conf (word_conf with col_oracle := []) asm_conf =
-    (source_iconf, clos_iconf, bvl_iconf, data_conf, (reg_count, livesets_data_init), livesets_init)
-  ∧
-  icompile_to_livesets source_iconf clos_iconf bvl_iconf data_conf (word_conf with col_oracle := []) asm_conf p =
-    SOME (source_iconf', clos_iconf', bvl_iconf', livesets_data_ic, icompiled_p_livesets)
-  ∧
-  end_icompile_to_livesets source_iconf' source_conf
-                           clos_iconf' clos_conf
-                           bvl_iconf' bvl_conf
-                           data_conf (word_conf with col_oracle := []) asm_conf
-  = (source_conf_after_ic, clos_conf_after_ic, bvl_conf_after_ic, livesets_data_end, livesets_end)
-  ∧
-  to_livesets_alt source_conf clos_conf bvl_conf data_conf (word_conf with col_oracle := []) asm_conf p =
-    (source_conf_after_c, clos_conf_after_c, bvl_conf_after_c, (reg_count_c, livesets_data_c), compiled_p)
-  ∧
-  source_conf = source_to_flat$empty_config
-  ∧
-  clos_conf = clos_to_bvl$default_config
-  ∧
-  bvl_conf = bvl_to_bvi$default_config
-  ∧
-  stack_conf_init stack_conf
-  ⇒
-  config_prog_rel_livesets     source_conf_after_ic source_conf_after_c
-                               clos_conf_after_c clos_conf_after_ic
-                               bvl_conf_after_ic bvl_conf_after_c
-                               reg_count reg_count_c
-                               (livesets_data_init ++ livesets_data_ic ++ livesets_data_end) livesets_data_c
-                               (livesets_init ++ icompiled_p_livesets ++ livesets_end) compiled_p
+Theorem icompile_icompile_source_to_livesets:
+  icompile_source_to_livesets asm_conf ic p1 = SOME (ic', d1, p1') ∧
+  icompile_source_to_livesets asm_conf ic' p2 = SOME (ic'', d2, p2') ⇒
+  icompile_source_to_livesets asm_conf ic (p1 ++ p2) = SOME (ic'', d1 ++ d2, p1' ++ p2')
 Proof
-  once_rewrite_tac[init_icompile_to_livesets_def, icompile_to_livesets_def, end_icompile_to_livesets_def, to_livesets_alt_def] >>
-  simp[] >>
-  strip_tac >>
-  ntac 4 (pop_assum mp_tac) >>
-  rpt (pairarg_tac >> fs[]) >>
-  qpat_x_assum ‘end_icompile_source_to_flat _ _ = _’ mp_tac >>
+  rw[icompile_source_to_livesets_def] >>
   gvs[AllCaseEqs()] >> rpt (pairarg_tac >> gvs[]) >>
-  rpt strip_tac >>
-  drule_all init_icompile_icompile_end_icompile_s2f >>
-  simp[config_prog_pair_rel_def] >>
-  strip_tac >>
-  pop_assum (fn f => assume_tac (GSYM f)) >>
-  qpat_x_assum ‘clos_conf = _ ’ mp_tac >>
-  qpat_x_assum ‘bvl_conf = _ ’ mp_tac >>
-  qpat_x_assum ‘clos_to_bvl_compile_alt _ _ = _ ’ mp_tac >> simp[] >>
-  strip_tac >>
-  drule_all init_icompile_icompile_end_icompile_f2c_alt >>
-  strip_tac >> pop_assum $ qspec_then ‘icompiled_p_flat’ assume_tac >>
-  gvs[] >>
-  rpt strip_tac >>
-  qpat_x_assum ‘bvl_conf = _ ’ mp_tac >>
-  drule_all init_icompile_icompile_end_icompile_c2b >>
-  simp[config_prog_pair_rel_def] >>
-  strip_tac >> qpat_x_assum ‘clos_conf = _’ mp_tac >>
-  gvs[] >> rpt strip_tac >>
-  drule_all init_icompile_icompile_end_icompile_b2b >>
-  simp[config_prog_rel_b2b_def] >>
-  strip_tac >>
-  rw[bvi_to_dataTheory.compile_prog_def] >> rw[] >>
-  ‘bvi_to_data$compile_prog (bvi_init ++ icompiled_p_bvi ++ bvi_end) =
-   bvi_to_data$compile_prog bvi_init ++
-   bvi_to_data$compile_prog icompiled_p_bvi ++
-   bvi_to_data$compile_prog bvi_end
-  ’ by rw[bvi_to_dataTheory.compile_prog_def] >> gvs[] >>
-  fs[data_to_wordTheory.compile_0_def] >>
-  fs[init_icompile_data_to_word_def, icompile_data_to_word_def] >>
-  gvs[] >>
-  qpat_x_assum ‘to_livesets_0_alt _ _  = (_, livesets_init)’
-               (fn th => assume_tac th >> drule to_livesets_0_alt_append) >>
-  disch_then (fn th =>
-                qpat_x_assum ‘to_livesets_0_alt _ _ = (_, icompiled_p_livesets)’ assume_tac >>
-              drule th) >>
-  strip_tac >>
-  drule to_livesets_0_alt_append >>
-  disch_then (fn th =>
-                qpat_x_assum ‘to_livesets_0_alt _ _ = (_, livesets_end)’ assume_tac >>
-              drule th) >>
-  rw[config_prog_rel_livesets]
-QED
-
-
-(* Repeated, maybe can find a way to reuse ? *)
-Theorem icompile_to_livesets_none:
-  icompile_to_livesets a b c d e f p = NONE ⇒
-  icompile_to_livesets a b c d e f (p ++ p') = NONE
-Proof
-  rw[icompile_to_livesets_def, source_to_source_compile_append] >>
-  rw[icompile_icompile_source_to_flat] >>
-  Cases_on ‘icompile_source_to_flat a (compile p)’
-  >- (gvs[] >> drule icompile_icompile_source_to_flat_none >> rw[])
-  >- (Cases_on ‘x’ >>
-      gvs[] >> rpt (pairarg_tac >> gvs[]))
-QED
-
-Theorem icompile_to_livesets_none1:
-  icompile_to_livesets a b c d e f p = SOME (a', b', c', g', _) ∧
-  icompile_to_livesets a' b' c' d' e f p'  = NONE ⇒
-  icompile_to_livesets a b c d e f (p ++ p') = NONE
-Proof
-  rw[icompile_to_livesets_def, source_to_source_compile_append] >>
-  Cases_on ‘icompile_source_to_flat a (compile p)’ >> gvs[] >>
-  namedCases_on ‘x’ ["a' b'"] >> gvs[] >>
-  rpt (pairarg_tac >> gvs[]) >>
-  Cases_on ‘icompile_source_to_flat a' (compile p')’
-  >- (gvs[icompile_icompile_source_to_flat_none1])
-  >- (namedCases_on ‘x’ ["a'' b''"] >> gvs[] >> rpt (pairarg_tac >> gvs[]))
-QED
-
-Theorem fold_icompile_to_livesets_collapse:
-  ∀pss source_iconf clos_iconf bvl_iconf data_conf word_conf asm_conf .
-  fold_icompile_to_livesets source_iconf clos_iconf bvl_iconf data_conf (word_conf with col_oracle := []) asm_conf pss  =
-  icompile_to_livesets source_iconf clos_iconf bvl_iconf data_conf (word_conf with col_oracle := []) asm_conf (FLAT pss)
-Proof
-  Induct >> rw[fold_icompile_to_livesets_def] >>
-  Cases_on ‘icompile_to_livesets source_iconf clos_iconf bvl_iconf data_conf (word_conf with col_oracle := []) asm_conf h’
-  >- (simp[] >> drule icompile_to_livesets_none >> rw[])
-  >- (namedCases_on ‘x’ ["source_iconf' clos_iconf' bvl_iconf' livesets_data' p'"] >>
-      rw[] >>
-      (Cases_on ‘icompile_to_livesets source_iconf' clos_iconf' bvl_iconf' data_conf (word_conf with col_oracle := []) asm_conf (FLAT pss)’
-       >- (simp[] >> drule icompile_to_livesets_none1 >> disch_then drule >> rw[])
-       >- (namedCases_on ‘x’ ["source_iconf'' clos_iconf'' bvl_iconf'' livesets_data'' ps'"] >>
-           simp[] >> rev_drule_all icompile_icompile_to_livesets >> rw[])))
-QED
-
-
-Theorem to_livesets_0_alt_append:
-  to_livesets_0_alt asm_conf (word_conf, p1) = ((a, data1), p1') ∧
-  to_livesets_0_alt asm_conf (word_conf, p2) = ((_, data2), p2') ⇒
-  to_livesets_0_alt asm_conf (word_conf, (p1 ++ p2)) = ((a, data1 ++ data2), p1' ++ p2')
-Proof
-  rw[to_livesets_0_alt_def]
-QED
-
-
-Theorem icompile_icompile_to_livesets:
-  icompile_to_livesets source_iconf clos_iconf bvl_iconf
-                       data_conf (word_conf with col_oracle := []) asm_conf p1 =
-  SOME (source_iconf', clos_iconf', bvl_iconf', data1, p1')
-  ∧
-  icompile_to_livesets source_iconf' clos_iconf' bvl_iconf'
-                       data_conf (word_conf with col_oracle := []) asm_conf p2 =
-  SOME (source_iconf'', clos_iconf'', bvl_iconf'', data2, p2')
-  ⇒
-  icompile_to_livesets source_iconf clos_iconf bvl_iconf
-                       data_conf (word_conf with col_oracle := []) asm_conf (p1 ++ p2) =
-  SOME (source_iconf'', clos_iconf'', bvl_iconf'', data1 ++ data2, p1' ++ p2')
-Proof
-  rw[] >>
-  gvs[icompile_to_livesets_def] >> rpt (pairarg_tac >> gvs[]) >> rw[source_to_source_compile_append] >>
-  gvs[AllCaseEqs()] >> rpt (pairarg_tac >> gvs[]) >>
+  rw[source_to_source_compile_append] >>
   drule_all icompile_icompile_source_to_flat >> strip_tac >> gvs[] >>
-  fs[icompile_flat_to_clos_and_append_commute] >>
+  rpt (pairarg_tac >> gvs[]) >>
+  gvs[icompile_flat_to_clos_and_append_commute] >>
   rev_drule_all icompile_icompile_clos_to_bvl_alt >>
-  rpt (strip_tac >> gvs[]) >>
+  strip_tac >> gvs[] >>
   drule_all icompile_icompile_bvl_to_bvi >>
-  rpt (strip_tac >> gvs[]) >>
-  rw[bvi_to_dataTheory.compile_prog_def] >> pairarg_tac >> simp[] >>
-  pop_assum mp_tac >>
+  strip_tac >> gvs[] >>
+  simp[bvi_to_dataTheory.compile_prog_def] >>
   simp[icompile_icompile_data_to_word] >>
-  drule to_livesets_0_alt_append >> disch_then rev_drule >>
-  simp[bvi_to_dataTheory.compile_prog_def]
+  qpat_x_assum ‘word0_to_livesets _ _ = ((_, d1), _)’ assume_tac >>
+  drule word0_to_livesets_append >>
+  qpat_x_assum ‘word0_to_livesets _ _ = ((_, d2), _)’ assume_tac >>
+  disch_then drule >>
+  gvs[bvi_to_dataTheory.compile_prog_def] >>
+  gvs[icompile_icompile_data_to_word]
 QED
 
+Definition fold_icompile_source_to_livesets_def:
+  fold_icompile_source_to_livesets asm_conf ic [] =
+    icompile_source_to_livesets asm_conf ic []
+  ∧
+  fold_icompile_source_to_livesets asm_conf ic (p :: ps)  =
+  case icompile_source_to_livesets asm_conf ic p of NONE => NONE
+  | SOME (ic', d, p') =>
+    (case fold_icompile_source_to_livesets asm_conf ic' ps of NONE => NONE
+    | SOME (ic'', d', ps') =>
+      SOME (ic'', d ++ d', p' ++ ps'))
+End
 
-Theorem icompile_to_livesets_eq:
-  init_icompile_to_livesets source_conf clos_conf bvl_conf data_conf (word_conf with col_oracle := []) asm_conf  =
-    (source_iconf, clos_iconf, bvl_iconf, data_conf, (reg_count, livesets_data_init), livesets_init)
+
+Theorem icompile_source_to_livesets_none:
+  (icompile_source_to_livesets asm_conf ic p = NONE ⇒
+   icompile_source_to_livesets asm_conf ic (p ++ p') = NONE)
   ∧
-  fold_icompile_to_livesets source_iconf clos_iconf bvl_iconf data_conf (word_conf with col_oracle := []) asm_conf pss =
-    SOME (source_iconf', clos_iconf', bvl_iconf', livesets_data_ic, icompiled_p_livesets)
-  ∧
-  end_icompile_to_livesets source_iconf' source_conf
-                           clos_iconf' clos_conf
-                           bvl_iconf' bvl_conf
-                           data_conf (word_conf with col_oracle := []) asm_conf
-  = (source_conf_after_ic, clos_conf_after_ic, bvl_conf_after_ic, livesets_data_end, livesets_end)
-  ∧
-  to_livesets_alt source_conf clos_conf bvl_conf data_conf (word_conf with col_oracle := []) asm_conf (FLAT pss) =
-    (source_conf_after_c, clos_conf_after_c, bvl_conf_after_c, (reg_count_c, livesets_data_c), compiled_p)
-  ∧
-  source_conf = source_to_flat$empty_config
-  ∧
-  clos_conf = clos_to_bvl$default_config
-  ∧
-  bvl_conf = bvl_to_bvi$default_config
-  ∧
-  stack_conf_init stack_conf
-  ⇒
-  config_prog_rel_livesets     source_conf_after_ic source_conf_after_c
-                               clos_conf_after_c clos_conf_after_ic
-                               bvl_conf_after_ic bvl_conf_after_c
-                               reg_count reg_count_c
-                               (livesets_data_init ++ livesets_data_ic ++ livesets_data_end) livesets_data_c
-                               (livesets_init ++ icompiled_p_livesets ++ livesets_end) compiled_p
+  (icompile_source_to_livesets asm_conf ic p = SOME (ic', some_p) ∧
+   icompile_source_to_livesets asm_conf ic' p' = NONE ⇒
+   icompile_source_to_livesets asm_conf ic (p ++ p') = NONE)
 Proof
-  once_rewrite_tac[fold_icompile_to_livesets_collapse] >>
-  metis_tac[init_icompile_icompile_end_icompile_to_livesets]
+  once_rewrite_tac [icompile_source_to_livesets_def] >>
+  simp[source_to_source_compile_append] >>
+  Cases_on ‘icompile_source_to_flat ic.source_iconf (compile p)’ >> simp[]
+  >- (drule icompile_icompile_source_to_flat_none >> strip_tac >> gvs[])
+  >- (namedCases_on ‘x’ ["source_iconf' icompiled_p_flat"] >> simp[] >>
+      rpt (pairarg_tac >> gvs[]) >> strip_tac >>
+      Cases_on ‘icompile_source_to_flat ic'.source_iconf (compile p')’ >> gvs[]
+      >- (drule_all icompile_icompile_source_to_flat_none1  >> rw[])
+      >- (every_case_tac >> gvs[] >> rpt (pairarg_tac >> gvs[])))
 QED
+
+
+Theorem fold_icompile_source_to_livesets_collapse:
+  ∀pss ic.
+    fold_icompile_source_to_livesets asm_conf ic pss =
+    icompile_source_to_livesets asm_conf ic (FLAT pss)
+Proof
+  Induct >> rw[fold_icompile_source_to_livesets_def] >>
+  Cases_on ‘icompile_source_to_livesets asm_conf ic h’ >> gvs[]
+  >- (drule $ CONJUNCT1 icompile_source_to_livesets_none >> rw[])
+  >- (namedCases_on ‘x’ ["ic' d p'"] >> simp[] >>
+      Cases_on ‘icompile_source_to_livesets asm_conf ic' (FLAT pss)’ >> simp[]
+      >- (drule $ CONJUNCT2 icompile_source_to_livesets_none >> rw[])
+      >- (namedCases_on ‘x’ ["ic'' d' ps'"] >> simp[] >>
+          drule_all icompile_icompile_source_to_livesets >>
+          rw[]))
+QED
+
+Definition config_prog_rel4_def:
+  config_prog_rel4 c1 c2 p1 p2 d1 d2 rc1 rc2=
+  (c1 = c2 ∧ p1 = p2 ∧ d1 = d2 ∧ rc1 = rc2)
+End
+
+Theorem init_icompile_icompile_end_icompile_s2lvs:
+  init_icompile_source_to_livesets asm_conf c = (ic, (reg_count_ic, d_init), word0_init)
+  ∧
+  icompile_source_to_livesets asm_conf ic p = SOME (ic', d_ic, icompiled_p)
+  ∧
+  end_icompile_source_to_livesets asm_conf ic' c = (c_after_ic, d_end, word0_end)
+  ∧
+  source_to_livesets asm_conf c p = (c_after_c, (reg_count_c, d_c), compiled_p)
+  ∧
+  conf_ok c ⇒
+  config_prog_rel4 c_after_ic c_after_c
+                   (word0_init ++ icompiled_p ++ word0_end) compiled_p
+                   (d_init ++ d_ic ++ d_end) d_c
+                   reg_count_ic reg_count_c
+Proof
+  rw[init_icompile_source_to_livesets_def,
+     icompile_source_to_livesets_def,
+     end_icompile_source_to_livesets_def,
+     source_to_livesets_def,
+     source_to_word0_def,
+     conf_ok_def] >>
+  gvs[AllCaseEqs()] >> rpt (pairarg_tac >> gvs[]) >>
+  drule_all init_icompile_icompile_end_icompile_s2f >>
+  simp[config_prog_pair_rel_def] >> strip_tac >>
+  gvs[] >>
+  drule_all init_icompile_icompile_end_icompile_f2c_alt >>
+  strip_tac >> gvs[] >>
+  drule_all init_icompile_icompile_end_icompile_c2b >>
+  simp[config_prog_pair_rel_def] >> strip_tac >>
+  gvs[] >>
+  drule_all init_icompile_icompile_end_icompile_b2b >>
+  simp[config_prog_rel_b2b_def] >> strip_tac >> gvs[] >>
+  gvs[bvi_to_data_prog_compile_append_all] >>
+  drule init_icompile_icompile_end_icompile_d2w0 >> strip_tac >> gvs[] >>
+  qpat_x_assum ‘word0_to_livesets _ _ = ((_, d_init), _)’ assume_tac >>
+  drule word0_to_livesets_append >>
+  qpat_x_assum ‘word0_to_livesets _ _ = ((_, d_ic), _)’ assume_tac >>
+  disch_then drule >> strip_tac >>
+  drule word0_to_livesets_append >>
+  qpat_x_assum ‘word0_to_livesets _ _ = ((_, d_end), _)’ assume_tac >>
+  disch_then drule  >>
+  strip_tac >> gvs[] >>
+  simp[config_prog_rel4_def]
+QED
+
+Theorem icompile_eq_s2livesets:
+  init_icompile_source_to_livesets asm_conf c = (ic, (reg_count_ic, d_init), word0_init)
+  ∧
+  fold_icompile_source_to_livesets asm_conf ic p = SOME (ic', d_ic, icompiled_p)
+  ∧
+  end_icompile_source_to_livesets asm_conf ic' c = (c_after_ic, d_end, word0_end)
+  ∧
+  source_to_livesets asm_conf c (FLAT p) = (c_after_c, (reg_count_c, d_c), compiled_p)
+  ∧
+  conf_ok c ⇒
+  config_prog_rel4 c_after_ic c_after_c
+                   (word0_init ++ icompiled_p ++ word0_end) compiled_p
+                   (d_init ++ d_ic ++ d_end) d_c
+                   reg_count_ic reg_count_c
+Proof
+  once_rewrite_tac[fold_icompile_source_to_livesets_collapse] >>
+  metis_tac[init_icompile_icompile_end_icompile_s2lvs]
+QED
+
 
 
 val _ = export_theory();
